&emsp;
# Derivatives of inverse trig functions
# $\sin^{-1}(u) = \frac{1}{{\sqrt{ 1-u^2 }}} \frac{du}{dx}$
---
# $\cos^{-1}(u)=\frac{-1}{\sqrt{ 1-u^2 }}\frac{du}{dx}$
---
# $\tan^{-1}(u)=\frac{1}{1+u^2} \frac{du}{dx}$
---
# $\sec^{-1}(u) = \frac{1}{|u|\sqrt{ u^2 -1}}\frac{du}{dx}$
---
# $\cot^{-1}(u) =\frac{{-1}}{1+u^2}\frac{du}{dx}$
---
# $\csc^{-1}(u) = \frac{{-1}}{|u|\sqrt{ u^2-1 }}\frac{du}{dx}$
---
&emsp;
# Derivatives of inverse functions
$$[f(f^{-1}(x))]^{'} =[x]^{'} \rightarrow f'(f^{-1}(x)) * [f^{-1}(x)]^{'}=1$$

---
&emsp;
# Inverse functions 
$$f(a)=b \rightarrow f^{-1}(b)=a$$
This basically means that we can reverse the logic here and input different values 

---
&emsp;
# Identity
$$[f^{-1}(x)]^{'}=\frac{1}{g'(f^{-1}(x))}$$


---
&emsp;
# Resources 
