## vid notes 
[video link ](https://www.youtube.com/watch?v=xbviQHhU1rA)


### Dump

- every time you differentiate a y variable you must add $\frac{dy}{dx}$
- isolate $\frac{dy}{dx}$ to one side
- Divide the side that doesn't contain $\frac{dy}{dx}$ by the side that contains $\frac{dy}{dx}$.
	- This works because you can factor out the $\frac{dy}{dx}$ and then divide whatever is left to the other side 
	- Example of the Rule starting with:  $a\frac{dy}{dx} + b\frac{dy}{dx}  = c$
	- First factor out $\frac{dy}{dx}$ :    $\frac{dy}{dx}(a+b) = c$
	- Then divide $(a+b)$ on both sides:  $\frac{\frac{dy}{dx}\cancel{(a+b)}}{\cancel{(a+b)}} = \frac{c}{(a+b)}$ to get: $\frac{dy}{dx} = \frac{c}{a+b}$  
	- The solution is there for  $\frac{dy}{dx} = \frac{c}{a+b}$  


# 