
#workInProgress
## Why does it work?
The formulas of Trigonometric Substitution are substitutes because they do the same action as the trig function making them equal. The formulas are often similar to solving for a side of a triangle and can be derived from [[Pythagoras theorem]] $(a^2+b^2=c^2)$. [Further explanation](https://youtu.be/EV5dhv0A2wU?t=14)
## Formulas 
$$
\int \sqrt{ a^2-x^2 } \, dx  \to x= a\sin(\theta)
$$
$$
\int \sqrt{a^2+x^2 } \, dx  \to x = a\tan(\theta)
$$
$$
\int \sqrt{ x^2 -a^2} \, dx \to x= a\sec(\theta)
$$
&emsp;
&emsp;



# DUMP

## Class 
- Start with the  triangle and work backwords to simplyfy the  process of taking the trig function after solving and simplyfying. 

## Taking trig integrals

$\int  \sin^2(x)\cos^3(x) \, dx$
- Use trig identities to convert the equation into  on that you can integrate using [[U-Substitution|u sub]].
- Do this by reducing the odd trig function so it has a power of 1 this then allows you to take the [[U-Substitution|u sub]] 
$$\int  \sin^2(x)\cos^5(x) \, dx = \sin^2(1-\sin^2x)^2\cos x$$
