


# Dump

## Expansion
- Write the fraction as a expression as the sum of 2 rational expressions with a lower degree in the denominator.
- Again we want a higher degree in the original denominator
- factor the denominator of the original rational expression 
- Expand it for each factor?
- after expanding for each factor we want to multiply the numerator by the common denominator 
- can distribute the coefficients of the several rational expressions and then solve for a system of equations.

- First expand by each factor 
- Then multiply by the denominator of the original function which should be the common denominator.
- when the factor has a heigher degree than 1 we set the numorator of that compositon to $Ax+B$ so if we had factors of $\frac{1}{(x-1)(x^2+2x-7)}$ we would decompose those as $\frac{A}{(x-1)}+\frac{{Bx-C}}{x^2+2x-7}$
- Make sure to look for difference of squares when solving, but also remember that difference of squares is $(a^2-b^2)$ not $(a^2+b^2)$

[PFD CALCULATOR](https://www.emathhelp.net/en/calculators/algebra-2/partial-fraction-decomposition-calculator/?numer=6x-11&denom=%28x-1%29%5E2)
**Integration**
- Just do normal decomposition and then take the integral of the separated rational expressions
- $\int \frac{a}{x}+\frac{b}{x+2} \, dx =\int \frac{a}{x} \, dx +\int \frac{b}{x+2} \, dx$





---
<iframe width="560" height="315" src="https://www.youtube.com/embed/7IkufOBIw5g?si=F34M77X0Oz2DQOZy" title="YouTube video player" frameborder="0" allow="accelerometer; autoplay; clipboard-write; encrypted-media; gyroscope; picture-in-picture; web-share" referrerpolicy="strict-origin-when-cross-origin" allowfullscreen></iframe>
<iframe width="560" height="315" src="https://www.youtube.com/embed/S-XKGBesRzk?si=IfXyupPXF4cxln67" title="YouTube video player" frameborder="0" allow="accelerometer; autoplay; clipboard-write; encrypted-media; gyroscope; picture-in-picture; web-share" referrerpolicy="strict-origin-when-cross-origin" allowfullscreen></iframe>